gravy/src/org/gravy/checker/AbstractChecker.java
@@ -4,15 +4,26 @@
 package org.gravy.checker;
 
 import java.util.Collection;
+import java.util.HashMap;
 import java.util.HashSet;
+import java.util.LinkedHashMap;
+import java.util.LinkedList;
+import java.util.Map.Entry;
 
 import org.gravy.prover.Prover;
+import org.gravy.prover.ProverExpr;
 import org.gravy.prover.ProverFactory;
+import org.gravy.prover.ProverResult;
+import org.gravy.prover.princess.PrincessProver;
 import org.gravy.verificationcondition.AbstractTransitionRelation;
 import org.gravy.verificationcondition.CfgTransitionRelation;
+import org.joogie.cfgPlugin.Util.Dag;
+
 import util.Log;
+import ap.parser.IFormula;
 import boogie.controlflow.AbstractControlFlowFactory;
 import boogie.controlflow.BasicBlock;
+import boogie.controlflow.CfgAxiom;
 import boogie.controlflow.CfgProcedure;
 import boogie.statement.Statement;
 
@@ -78,4 +89,120 @@ public abstract class AbstractChecker implements Runnable {
 		this.prover = null;	
 	}
 
+	
+	
+	protected void pushTransitionRelation(Prover prover, AbstractTransitionRelation tr) {
+		//now assert all proof obligations
+		for (Entry<CfgAxiom, ProverExpr> entry : tr.getPreludeAxioms().entrySet()) {
+			prover.addAssertion(entry.getValue());
+		}
+		
+		prover.addAssertion(tr.getRequires());
+		
+        for (Entry<BasicBlock, LinkedList<ProverExpr>> entry : tr.getProofObligations()
+            .entrySet()) {
+          for (ProverExpr assertion : entry.getValue()) {
+            prover.addAssertion(assertion);
+          }
+        }
+	}
+
+	/**
+	 * Computes a maximal feasible path cover for the BasicBlocks 
+	 * in blocks2cover and returns the set of all covered nodes.
+	 * @param prover
+	 * @param tr
+	 * @param ineffFlags flags for the effectual blocks in blocks2cover
+	 * @param blocks2cover set of nodes for which the cover can be computed
+	 * @return subset of nodes in block2cover that can be covered.
+	 */
+	protected Collection<BasicBlock> computePathCover(Prover prover, CfgTransitionRelation tr,
+			LinkedHashMap<ProverExpr, ProverExpr> ineffFlags, HashSet<BasicBlock> blocks2cover) {
+
+		Dag<IFormula> vcdag = tr.getProverDAG();
+
+		HashSet<BasicBlock> coveredBlocks = new HashSet<BasicBlock>();
+		
+		// construct the inverted reachabilityVariables which is used later
+		// to keep track of what has been covered so far.
+		LinkedHashMap<ProverExpr, BasicBlock> uncoveredBlocks = new LinkedHashMap<ProverExpr, BasicBlock>();
+		for (Entry<BasicBlock, ProverExpr> entry : tr
+				.getReachabilityVariables().entrySet()) {
+			if (blocks2cover.contains(entry.getKey())) {
+				//ignore the blocks that we are not interested in
+				uncoveredBlocks.put(entry.getValue(), entry.getKey());
+			}	
+		}
+
+		int rounds = 0;
+		int threshold = ineffFlags.size();
+		// hint for the greedy cover algorithm about
+		// how many blocks could be covered in one query.
+		if (threshold > 1)
+			threshold = threshold / 2;
+
+		while (threshold >= 1 && !ineffFlags.isEmpty()) {
+			prover.push();
+
+			// setup the CFG module
+			LinkedList<ProverExpr> remainingBlockVars = new LinkedList<ProverExpr>();
+			LinkedList<ProverExpr> remainingIneffFlags = new LinkedList<ProverExpr>();
+			for (Entry<ProverExpr, ProverExpr> entry : ineffFlags.entrySet()) {
+				remainingBlockVars.add(entry.getKey());
+				remainingIneffFlags.add(entry.getValue());
+			}
+
+			((PrincessProver) prover).setupCFGPlugin(vcdag, remainingBlockVars,
+					remainingIneffFlags, threshold);
+
+			// Query the feasible paths for this setup
+			ProverResult res = prover.checkSat(true);
+
+			Log.debug("Round " + (rounds++));
+			Log.debug("Prover returns " + res.toString());
+
+			while (res == ProverResult.Sat) {
+				LinkedList<ProverExpr> covered = new LinkedList<ProverExpr>();
+				LinkedList<ProverExpr> flagsToAssert = new LinkedList<ProverExpr>();
+
+				for (Entry<ProverExpr, BasicBlock> entry : uncoveredBlocks
+						.entrySet()) {
+					final ProverExpr pe = entry.getKey();
+					if (prover.evaluate(pe).getBooleanLiteralValue()) {
+						covered.add(pe);
+						ProverExpr flag = ineffFlags.get(pe);
+						if (flag != null)
+							flagsToAssert.add(flag);
+					}
+				}
+
+				for (ProverExpr e : covered) {
+					ineffFlags.remove(e);
+					coveredBlocks.add(uncoveredBlocks.get(e) );
+					uncoveredBlocks.remove(e);
+				}
+
+				prover.addAssertion(prover.mkAnd(flagsToAssert
+						.toArray(new ProverExpr[flagsToAssert.size()])));
+
+				res = prover.checkSat(true);
+
+				Log.debug("Round " + (rounds++));
+				Log.debug("Prover returns " + res.toString());
+			}
+
+			prover.pop();
+
+			if (threshold == 1 || ineffFlags.isEmpty())
+				break;
+
+			do {
+				threshold = (int) Math.ceil((double) threshold / 2.0);
+			} while (threshold > ineffFlags.size());
+
+		}
+		return coveredBlocks;
+	}
+	
+	
 }
