gravy/src/org/gravy/checker/GravyChecker.java
@@ -3,21 +3,16 @@
  */
 package org.gravy.checker;
 
-import java.util.HashMap;
 import java.util.HashSet;
 import java.util.LinkedHashMap;
 import java.util.LinkedList;
-import java.util.Map.Entry;
 
 import org.gravy.Options;
 import org.gravy.callunwinding.CallUnwinding;
 import org.gravy.loopunwinding.AbstractLoopUnwinding;
-import org.gravy.loopunwinding.SimpleUnwinding;
 import org.gravy.prover.Prover;
 import org.gravy.prover.ProverExpr;
 import org.gravy.prover.ProverFactory;
-import org.gravy.prover.ProverResult;
-import org.gravy.prover.princess.PrincessProver;
 import org.gravy.ssa.SingleStaticAssignment;
 import org.gravy.verificationcondition.AbstractTransitionRelation;
 import org.gravy.verificationcondition.CfgTransitionRelation;
@@ -27,7 +22,6 @@ import util.Log;
 import ap.parser.IFormula;
 import boogie.controlflow.AbstractControlFlowFactory;
 import boogie.controlflow.BasicBlock;
-import boogie.controlflow.CfgAxiom;
 import boogie.controlflow.CfgProcedure;
 import boogie.controlflow.CfgVariable;
 import boogie.controlflow.expression.CfgBinaryExpression;
@@ -44,23 +38,22 @@ import boogie.type.BoogieType;
 
 /**
  * @author martin
- *
+ * 
  */
-public class GravyChecker extends
-		AbstractChecker {
+public class GravyChecker extends AbstractChecker {
 
 	/**
 	 * @param cff
 	 * @param p
 	 */
-	public GravyChecker(AbstractControlFlowFactory cff,
-			CfgProcedure p) {
+	public GravyChecker(AbstractControlFlowFactory cff, CfgProcedure p) {
 		super(cff, p);
-		
-		p.pruneUnreachableBlocks();		
 
-		if (Options.v().getDebugMode()) p.toFile("cfg_"+p.getProcedureName()+".bpl");
-		
+		p.pruneUnreachableBlocks();
+
+		if (Options.v().getDebugMode())
+			p.toFile("cfg_" + p.getProcedureName() + ".bpl");
+
 		CallUnwinding cunwind = new CallUnwinding();
 		cunwind.unwindCalls(p);
 
@@ -68,278 +61,209 @@ public class GravyChecker extends
 
 		p.pruneUnreachableBlocks();
 
-		if (Options.v().getDebugMode())  p.toFile("loopfree_"+p.getProcedureName()+".bpl");
-		
-		//turn assertions into conditional choices.
+		if (Options.v().getDebugMode())
+			p.toFile("loopfree_" + p.getProcedureName() + ".bpl");
+
+		// turn assertions into conditional choices.
 		turnAssertionsIntoConditionals(p);
-		
+
 		SingleStaticAssignment ssa = new SingleStaticAssignment();
 		ssa.recomputeSSA(p);
 
 		p.pruneUnreachableBlocks();
+		
+		if (Options.v().getDebugMode())
+			p.toFile("final_" + p.getProcedureName() + ".bpl");
+		
 	}
 
-	
 	@Override
 	public void run() {
 		ProverFactory pf = new org.gravy.prover.princess.PrincessProverFactory();
-		//Prover prover = pf.spawnWithLog("lala");
+		// Prover prover = pf.spawnWithLog("lala");
 		this.prover = pf.spawn();
-		Log.debug("Compute Transition Relation "+this.procedure.getProcedureName());
-		//AbstractTransitionRelation tr = new TransitionRelation(this.procedure, this.cff, prover);
-		CfgTransitionRelation tr = new CfgTransitionRelation(this.procedure, this.cff, prover);
-		checkSat(prover, tr); 
+		Log.debug("Compute Transition Relation "
+				+ this.procedure.getProcedureName());
+		// AbstractTransitionRelation tr = new
+		// TransitionRelation(this.procedure, this.cff, prover);
+		CfgTransitionRelation tr = new CfgTransitionRelation(this.procedure,
+				this.cff, prover);
+		checkSat(prover, tr);
 		shutDownProver();
 	}
-	
-	
-	/* (non-Javadoc)
-	 * @see org.gravy.infeasiblecode.AbstractInfeasibleCodeDetection#checkSat(org.gravy.prover.Prover, org.gravy.verificationcondition.CfgTransitionRelation)
+
+
+	/*
+	 * (non-Javadoc)
+	 * 
+	 * @see
+	 * org.gravy.infeasiblecode.AbstractInfeasibleCodeDetection#checkSat(org
+	 * .gravy.prover.Prover,
+	 * org.gravy.verificationcondition.CfgTransitionRelation)
 	 */
 	@Override
-	public void checkSat(Prover prover,
-			AbstractTransitionRelation atr) {
+	public void checkSat(Prover prover, AbstractTransitionRelation atr) {
 
-		
-//		StopWatch firstcheck = StopWatch.getInstanceAndStart();
-//		StopWatch allchecks = StopWatch.getInstanceAndStart();
-		
-		CfgTransitionRelation tr = (CfgTransitionRelation)atr;
+		// StopWatch firstcheck = StopWatch.getInstanceAndStart();
+		// StopWatch allchecks = StopWatch.getInstanceAndStart();
+
+		CfgTransitionRelation tr = (CfgTransitionRelation) atr;
 		Dag<IFormula> vcdag = tr.getProverDAG();
-
+		
 		// generate ineff flags; this map is also used to keep
 		// track of the remaining uncovered blocks
 		LinkedHashMap<ProverExpr, ProverExpr> ineffFlags = new LinkedHashMap<ProverExpr, ProverExpr>();
 
 		for (BasicBlock block : tr.getEffectualSet()) {
 			ProverExpr v = tr.getReachabilityVariables().get(block);
-			ineffFlags.put(
-					v,
-					prover.mkVariable("" + v + "_flag",
-							prover.getBooleanType()));
+			ineffFlags.put(v, prover.mkVariable("" + v + "_flag",
+					prover.getBooleanType()));
 		}
-		
-		
-        //construct the inverted reachabilityVariables which is used later 
-        //to keep track of what has been covered so far.
-        HashMap<ProverExpr, BasicBlock> uncoveredBlocks = new HashMap<ProverExpr, BasicBlock>();
-        
-        //@Daniel: allBlocks is a local helper that we use the reconstruct feasible paths later
-        HashMap<ProverExpr, BasicBlock> allBlocks = new HashMap<ProverExpr, BasicBlock>();
-        
-        for (Entry<BasicBlock, ProverExpr> entry : tr.getReachabilityVariables().entrySet()) {
-            uncoveredBlocks.put(entry.getValue(), entry.getKey());
-            allBlocks.put(entry.getValue(), entry.getKey());
-        }       
-		
 
-		//now assert all proof obligations
-		for (Entry<CfgAxiom, ProverExpr> entry : tr.getPreludeAxioms().entrySet()) {
-			prover.addAssertion(entry.getValue());
-		}
-		
-		//TODO: introduce a flag to decide if we want to check preconditions.
-		prover.addAssertion(tr.getRequires());
-		
-        for (Entry<BasicBlock, LinkedList<ProverExpr>> entry : tr.getProofObligations()
-            .entrySet()) {
-          for (ProverExpr assertion : entry.getValue()) {
-            prover.addAssertion(assertion);
-          }
-        }
-    
+		this.pushTransitionRelation(prover, tr);	
 
+		HashSet<BasicBlock> blocks2cover = new HashSet<BasicBlock>(tr.getReachabilityVariables().keySet()); 
+		
 		// now exclude all feasible paths that may violate the postcondition
-        prover.push();
+		prover.push();
 		prover.addAssertion(tr.getEnsures());
+		//compute the feasible path cover under the given postcondition
+		feasibleBlocks = new HashSet<BasicBlock>(computePathCover(prover, tr, ineffFlags, blocks2cover));
+		blocks2cover.removeAll(feasibleBlocks);
 		
-        for (int checkPostcondition=0; checkPostcondition<2; checkPostcondition++) {
+		//now pop the postcondition.
+		prover.pop();
+		infeasibleBlocksUnderPost = new HashSet<BasicBlock>(computePathCover(prover, tr, ineffFlags, blocks2cover));	
 		
-          int threshold = ineffFlags.size();
-          // slightly better guess
-          if (threshold > 1)
-            threshold = threshold / 2;
-
-          int rounds = 1;// only for pretty printing
-
-          while (threshold >= 1 && !ineffFlags.isEmpty()) {
-            prover.push();
-
-			// setup the CFG module
-			LinkedList<ProverExpr> remainingBlockVars = new LinkedList<ProverExpr>();
-			LinkedList<ProverExpr> remainingIneffFlags = new LinkedList<ProverExpr>();
-
-			for (Entry<ProverExpr, ProverExpr> entry : ineffFlags.entrySet()) {
-				remainingBlockVars.add(entry.getKey());
-				remainingIneffFlags.add(entry.getValue());
-			}
-
-			((PrincessProver) prover).setupCFGPlugin(vcdag,
-					remainingBlockVars, remainingIneffFlags, threshold);
-
-			// Query the feasible paths for this setup
-			ProverResult res = prover.checkSat(true);
-			//if (rounds==1) firstcheck.stop();
-			Log.debug("Round " + (rounds++));
-			Log.debug("Prover returns " + res.toString());
-
-			while (res == ProverResult.Sat) {
-				LinkedList<ProverExpr> covered = new LinkedList<ProverExpr>();
-				LinkedList<ProverExpr> flagsToAssert = new LinkedList<ProverExpr>();
-				
-                for (Entry<ProverExpr, BasicBlock> entry : uncoveredBlocks.entrySet()) {
-                  final ProverExpr pe = entry.getKey();
-                  if (prover.evaluate(pe).getBooleanLiteralValue()) {                	  
-                    covered.add(pe);                    
-                    if (checkPostcondition == 0) {
-                        //if we are in the first iteration, this is a feasible block
-                        feasibleBlocks.add(entry.getValue());
-                    } else {
-                        infeasibleBlocksUnderPost.add(entry.getValue());
-                    }
-                    
-                    ProverExpr flag = ineffFlags.get(pe);
-                    if (flag != null)
-                      flagsToAssert.add(flag);
-                  }
-                }
-				
-				for (ProverExpr e : covered) {
-					ineffFlags.remove(e);
-					uncoveredBlocks.remove(e);
-				}
-				
-				prover.addAssertion(prover.mkAnd(flagsToAssert
-						.toArray(new ProverExpr[flagsToAssert.size()])));
-
-				res = prover.checkSat(true);
-
-				Log.debug("Round " + (rounds++));
-				Log.debug("Prover returns " + res.toString());
-			}
-
-			prover.pop();
-
-			if (threshold == 1 || ineffFlags.isEmpty())
-				break;
-
-			do {
-			  threshold = (int) Math.ceil((double) threshold / 2.0);
-			} while (threshold > ineffFlags.size());
-			
-          }
-          
-          if (checkPostcondition == 1)
-            break;
-          
-          infeasibleBlocks.addAll(uncoveredBlocks.values());
-                    
-          //pop the assertion $ex_returned == false
-          prover.pop();
-        }
-		//allchecks.stop();
-		infeasibleBlocks = new HashSet<BasicBlock>();
-		infeasibleBlocks.addAll(uncoveredBlocks.values());
-
+		infeasibleBlocks = new HashSet<BasicBlock>(tr.getReachabilityVariables().keySet());
+		infeasibleBlocks.removeAll(feasibleBlocks);
+		infeasibleBlocks.removeAll(infeasibleBlocksUnderPost);
+		
 		StringBuilder sb = new StringBuilder();
-		sb.append("Statistics for "+this.procedure.getProcedureName() + " \n");
-		sb.append("Total Blocks: " + tr.getReachabilityVariables().size() + "\n");
+		sb.append("Statistics for " + this.procedure.getProcedureName() + " \n");
+		sb.append("Total Blocks: " + tr.getReachabilityVariables().size()
+				+ "\n");
 		sb.append("Feasible Blocks: " + feasibleBlocks.size() + "\n");
-		sb.append("Feasible Exceptional Blocks: " + infeasibleBlocksUnderPost.size()+"\n");
-		sb.append("Infeasible Blocks: " + uncoveredBlocks.size()+"\n");
+
+		sb.append("Feasible Exceptional Blocks: "
+				+ infeasibleBlocksUnderPost.size() + "\n");
 		
+		sb.append("Infeasible Blocks: " + infeasibleBlocks.size() + "\n");
+
 		int feasibleExceptions = 0;
 		for (BasicBlock b : infeasibleBlocksUnderPost) {
 			if (b.getLabel().endsWith("#assertionElse")) {
 				feasibleExceptions++;
 			}
 		}
-		
+
 		int infeasibleExceptions = 0;
 		for (BasicBlock b : infeasibleBlocks) {
 			if (b.getLabel().endsWith("#assertionElse")) {
 				infeasibleExceptions++;
 			}
 		}
-		
-		//TODO: this is a very primitive way of counting.
-		sb.append("feasibleExceptions: " + feasibleExceptions+"\n");
-		sb.append("infeasibleExceptions: " + infeasibleExceptions+"\n");
-		
+
+		// TODO: this is a very primitive way of counting.
+		sb.append("feasibleExceptions: " + feasibleExceptions + "\n");
+		sb.append("infeasibleExceptions: " + infeasibleExceptions + "\n");
+
 		Log.info(sb);
 	}
-
 
 	private void turnAssertionsIntoConditionals(CfgProcedure p) {
 		LinkedList<BasicBlock> todo = new LinkedList<BasicBlock>();
 		LinkedList<BasicBlock> done = new LinkedList<BasicBlock>();
 
 		if (!this.cff.getGlobalVars().containsKey("$$AssertionFailure")) {
-			this.cff.getGlobalVars().put("$$AssertionFailure", new CfgVariable("$$AssertionFailure", BoogieType.boolType, false, true, true, true ));			
+			this.cff.getGlobalVars().put(
+					"$$AssertionFailure",
+					new CfgVariable("$$AssertionFailure", BoogieType.boolType,
+							false, true, true, true));
 		}
-		CfgVariable asrtFail = this.cff.getGlobalVars().get("$$AssertionFailure");	
-		
-		
-		// add a postcondition to ensure that $$AssertionFailure is false before and
-		//after the execution of the procedure.
-		p.getEnsures().add(new CfgBinaryExpression(p.getLocation(), BoogieType.boolType, BinaryOperator.COMPEQ, 
-				new CfgIdentifierExpression(p.getLocation(), asrtFail), 
-				new CfgBooleanLiteral(p.getLocation(), BoogieType.boolType, false)));
-		
-		
-		//BFS throught the cfg and look for assertions.
+		CfgVariable asrtFail = this.cff.getGlobalVars().get(
+				"$$AssertionFailure");
+
+		// add a postcondition to ensure that $$AssertionFailure is false before
+		// and
+		// after the execution of the procedure.
+		p.getEnsures().add(
+				new CfgBinaryExpression(p.getLocation(), BoogieType.boolType,
+						BinaryOperator.COMPEQ, new CfgIdentifierExpression(p
+								.getLocation(), asrtFail),
+						new CfgBooleanLiteral(p.getLocation(),
+								BoogieType.boolType, false)));
+
+		// BFS throught the cfg and look for assertions.
 		todo.add(p.getRootNode());
 		while (!todo.isEmpty()) {
 			BasicBlock current = todo.removeLast();
 			done.add(current);
-			
-			for (CfgStatement stmt : new LinkedList<CfgStatement>(current.getStatements())) {
+
+			for (CfgStatement stmt : new LinkedList<CfgStatement>(
+					current.getStatements())) {
 				if (stmt instanceof CfgAssertStatement) {
-					CfgAssertStatement asrt = (CfgAssertStatement)stmt;
-					//if the block has an assertion, split the block in two, and replace 
-					//the assertion by a conditional choice.
+					CfgAssertStatement asrt = (CfgAssertStatement) stmt;
+					// if the block has an assertion, split the block in two,
+					// and replace
+					// the assertion by a conditional choice.
 					int splitIdx = current.getStatements().indexOf(stmt);
-					LinkedList<CfgStatement> prefix = new LinkedList<CfgStatement>(current.getStatements().subList(0, splitIdx));
-					LinkedList<CfgStatement> suffix = new LinkedList<CfgStatement>(current.getStatements().subList(splitIdx+1, current.getStatements().size()));
-					
-					BasicBlock thenBlock = new BasicBlock(asrt.getLocation(), current.getLabel()+"#assertionThen");
+					LinkedList<CfgStatement> prefix = new LinkedList<CfgStatement>(
+							current.getStatements().subList(0, splitIdx));
+					LinkedList<CfgStatement> suffix = new LinkedList<CfgStatement>(
+							current.getStatements().subList(splitIdx + 1,
+									current.getStatements().size()));
+
+					BasicBlock thenBlock = new BasicBlock(asrt.getLocation(),
+							current.getLabel() + "#assertionThen");
 					thenBlock.setStatements(suffix);
-					//add the condition of the assertion to the beginning of the then block
-					thenBlock.addStatement(new CfgAssumeStatement(asrt.getLocation(), asrt.getCondition()), true);
-					//shallow copy the successor and connect the blocks
-					HashSet<BasicBlock> succs = new HashSet<BasicBlock>(current.getSuccessors());
+					// add the condition of the assertion to the beginning of
+					// the then block
+					thenBlock.addStatement(
+							new CfgAssumeStatement(asrt.getLocation(), asrt
+									.getAttributes(), asrt.getCondition()),
+							true);
+					// shallow copy the successor and connect the blocks
+					HashSet<BasicBlock> succs = new HashSet<BasicBlock>(
+							current.getSuccessors());
 					for (BasicBlock succ : succs) {
 						thenBlock.connectToSuccessor(succ);
 						current.disconnectFromSuccessor(succ);
 					}
-					
-					BasicBlock elseBlock = new BasicBlock(asrt.getLocation(), current.getLabel()+"#assertionElse");
-					elseBlock.addStatement(new CfgAssumeStatement(asrt.getLocation(), 
-							new CfgUnaryExpression(asrt.getLocation(), 
-									asrt.getCondition().getType(), UnaryOperator.LOGICNEG, asrt.getCondition())
-					), true);
-					
-					elseBlock.addStatement(new CfgAssignStatement(asrt.getLocation(), 
-							new CfgIdentifierExpression(asrt.getLocation(), asrtFail),
-							new CfgBooleanLiteral(asrt.getLocation(), BoogieType.boolType, true)), false );
-					
-					
+
+					BasicBlock elseBlock = new BasicBlock(asrt.getLocation(),
+							current.getLabel() + "#assertionElse");
+					elseBlock.addStatement(
+							new CfgAssumeStatement(asrt.getLocation(), asrt
+									.getAttributes(), new CfgUnaryExpression(
+									asrt.getLocation(), asrt.getCondition()
+											.getType(), UnaryOperator.LOGICNEG,
+									asrt.getCondition())), true);
+
+					elseBlock.addStatement(
+							new CfgAssignStatement(asrt.getLocation(),
+									new CfgIdentifierExpression(asrt
+											.getLocation(), asrtFail),
+									new CfgBooleanLiteral(asrt.getLocation(),
+											BoogieType.boolType, true)), false);
+
 					current.setStatements(prefix);
 					current.connectToSuccessor(thenBlock);
 					current.connectToSuccessor(elseBlock);
-					//now set current to the suffix so that we can continue to look
-					//for more assertions.
+					// now set current to the suffix so that we can continue to
+					// look
+					// for more assertions.
 					current = thenBlock;
 				}
 			}
-			
-			if (current.getSuccessors().size()>0) {
+
+			if (current.getSuccessors().size() > 0) {
 				for (BasicBlock next : current.getSuccessors()) {
 					if (!todo.contains(next) && !done.contains(next)) {
 						todo.add(next);
 					}
 				}
-			} 		
-		}		
+			}
+		}
 	}
 }
