gravy_test/regression/gradual_verification/gradualverification001.bpl
@@ -1,219 +1,136 @@
-procedure void$org.joogie.tests.InfeasibleCodeSnippets$main$1867($in_parameter__0:ref) returns ($exception:ref)
-    modifies $heap, $stringSizeHeap;
-{
-    var $ex_return : bool;
-    var s10 : ref;
-    var $fakelocal_3 : ref;
-    var temp$011 : ref;
-    var temp$112 : ref;
-    var args9 : ref;
-    var $fakelocal_0 : ref;
-    var $fakelocal_2 : ref;
-    var $fakelocal_1 : ref;
-    var temp$213 : ref;
-
-    $ex_return := false;
-    args9 := $in_parameter__0;
-    havoc $fakelocal_0;
-    assume !$heap[$fakelocal_0,$alloc];
-    $heap := $heap[$fakelocal_0,$alloc := true];
-    assume $fakelocal_0 != $null;
-    $heap := $heap[$fakelocal_0,$type := java.lang.String];
-    $stringSizeHeap := $stringSizeHeap[$fakelocal_0 := 5];
-    s10 := $fakelocal_0;
-    if (s10 != $null) {
-        $exception := $exception;
-    } else {
-        havoc $fakelocal_1;
-        assume !$heap[$fakelocal_1,$alloc];
-        $heap := $heap[$fakelocal_1,$alloc := true];
-        assume $fakelocal_1 != $null;
-        $heap := $heap[$fakelocal_1,$type := java.lang.NullPointerException];
-        $exception := $fakelocal_1;
-        $ex_return := true;
-        return;
-    }
-    if ($heap[s10,$type] <: java.lang.String && java.lang.String <: $heap[s10,$type]) {
-        call temp$011, $exception := java.lang.String$java.lang.String$toLowerCase$120(s10);
-        assume temp$011 != $null;
-        assume $heap[temp$011,$type] <: java.lang.String;
-        assume java.lang.String <: $heap[temp$011,$type];
-    }
-    if (temp$011 != $null) {
-        $exception := $exception;
-    } else {
-        havoc $fakelocal_2;
-        assume !$heap[$fakelocal_2,$alloc];
-        $heap := $heap[$fakelocal_2,$alloc := true];
-        assume $fakelocal_2 != $null;
-        $heap := $heap[$fakelocal_2,$type := java.lang.NullPointerException];
-        $exception := $fakelocal_2;
-        $ex_return := true;
-        return;
-    }
-    if ($heap[temp$011,$type] <: java.lang.String && java.lang.String <: $heap[temp$011,$type]) {
-        call temp$112, $exception := java.lang.String$java.lang.String$substring$108(temp$011, 0, 1);
-        assume temp$112 != $null;
-        assume $heap[temp$112,$type] <: java.lang.String;
-        assume java.lang.String <: $heap[temp$112,$type];
-    }
-    if (temp$112 != $null) {
-        $exception := $exception;
-    } else {
-        havoc $fakelocal_3;
-        assume !$heap[$fakelocal_3,$alloc];
-        $heap := $heap[$fakelocal_3,$alloc := true];
-        assume $fakelocal_3 != $null;
-        $heap := $heap[$fakelocal_3,$type := java.lang.NullPointerException];
-        $exception := $fakelocal_3;
-        $ex_return := true;
-        return;
-    }
-    if ($heap[temp$112,$type] <: java.lang.String && java.lang.String <: $heap[temp$112,$type]) {
-        call temp$213, $exception := java.lang.String$java.lang.String$toUpperCase$122(temp$112);
-        assume temp$213 != $null;
-        assume $heap[temp$213,$type] <: java.lang.String;
-        assume java.lang.String <: $heap[temp$213,$type];
-    }
-    return;
+type ref;
+type javaType;
+type Field $GenericType__0;
+type $heap_type = <$GenericType__0>[ref,Field $GenericType__0]$GenericType__0;
+type boolArrHeap_type = [ref][int]bool;
+type refArrHeap_type = [ref][int]ref;
+type realArrHeap_type = [ref][int]int;
+type intArrHeap_type = [ref][int]int;
+const unique $null : ref;
+const unique $type : Field javaType;
+const unique $alloc : Field bool;
+const unique java.lang.Object : javaType extends  complete;
+const unique InfeasibleCode01 : javaType extends  unique java.lang.Object complete;
+var $heap : $heap_type;
+var $intArrayType : javaType;
+var $charArrayType : javaType;
+var $boolArrayType : javaType;
+var $byteArrayType : javaType;
+var $longArrayType : javaType;
+var $arrSizeHeap : [ref]int;
+var $stringSizeHeap : [ref]int;
+var $boolArrHeap : boolArrHeap_type;
+var $refArrHeap : refArrHeap_type;
+var $realArrHeap : realArrHeap_type;
+var $intArrHeap : intArrHeap_type;
+var InfeasibleCode01$InfeasibleCode01$bases234 : Field ref;
+function $arrayType(t:javaType) returns ($ret:javaType);
+function $intToReal(x:int) returns ($ret:real);
+function $intToBool(x:int) returns ($ret:bool) { (if x == 0 then false else true) }
+function $refToBool(x:ref) returns ($ret:bool) { (if x == $null then false else true) }
+function $boolToInt(x:bool) returns ($ret:int) { (if x == true then 1 else 0) }
+function $cmpBool(x:bool, y:bool) returns ($ret:int);
+function $cmpRef(x:ref, y:ref) returns ($ret:int);
+function $cmpReal(x:real, y:real) returns ($ret:int) { (if x > y then 1 else (if x < y then -1 else 0)) }
+function $cmpInt(x:int, y:int) returns ($ret:int) { (if x > y then 1 else (if x < y then -1 else 0)) }
+function $bitOr(x:int, y:int) returns ($ret:int);
+function $bitAnd(x:int, y:int) returns ($ret:int);
+function $xorInt(x:int, y:int) returns ($ret:int);
+function $shlInt(x:int, y:int) returns ($ret:int);
+function $ushrInt(x:int, y:int) returns ($ret:int);
+function $shrInt(x:int, y:int) returns ($ret:int);
+procedure java.lang.Object$java.lang.Object$clone$43($this:ref) returns ($other:ref, $exception:ref)    modifies $heap;{
+    havoc $other;
+    assume !$heap[$other,$alloc];
+    $heap := $heap[$other,$alloc := true];
+    assume $other != $null;
+    $heap := $heap[$other,$type := $heap[$this,$type]];
 }
 
-procedure int$org.joogie.tests.InfeasibleCodeSnippets$test1$1865($this:ref, $in_parameter__0:int) returns ($return:int, $exception:ref)
-    modifies ;
-{
-    var this1 : ref;
-    var y3 : int;
-    var x2 : int;
-    var temp$04 : int;
-    var $ex_return : bool;
-    var temp$15 : int;
 
+procedure int$java.lang.String$compareTo$87($this:ref, $other:ref) returns ($return:int, $exception:ref);    ensures ($this == $other ==> $return == 1) && ($this != $other ==> $return == 0);    
+
+procedure boolean$InfeasibleCode01$foo$1889($this:ref, $in_parameter__0:ref) returns ($return:int, $exception:ref);    
+
+procedure int$java.lang.Object$hashCode$41($this:ref) returns ($return:int, $exception:ref);    
+
+procedure void$InfeasibleCode01$$la$init$ra$$1890($this:ref) returns ($exception:ref);    
+
+procedure void$java.lang.Object$$la$init$ra$$38($this:ref) returns ($exception:ref);    
+
+implementation boolean$InfeasibleCode01$foo$1889($this:ref, $in_parameter__0:ref) returns ($return:int, $exception:ref){
+    
+var temp$36 : ref;    
+var this1 : ref;    
+var temp$58 : ref;    
+var temp$03 : ref;    
+var other2 : ref;    
+var temp$47 : int;    
+var $ex_return : bool;    
+var temp$25 : int;    
+var temp$69 : int;    
+var temp$811 : int;    
+var temp$14 : ref;    
+var temp$710 : int;
     assume $this != $null;
     $ex_return := false;
     this1 := $this;
-    x2 := $in_parameter__0;
-    y3 := 0;
-    temp$04 := y3;
-    temp$15 := temp$04 + x2;
-    $return := temp$15;
+    other2 := $in_parameter__0;
+    assert this1 != $null;
+    temp$03 := $heap[this1,InfeasibleCode01$InfeasibleCode01$bases234];
+    if (temp$03 == $null) {
+        goto block1;
+    }
+    goto block2;
+  block1:
+    assert other2 != $null;
+    temp$14 := $heap[other2,InfeasibleCode01$InfeasibleCode01$bases234];
+    if (temp$14 != $null) {
+        goto block3;
+    }
+    goto block4;
+  block3:
+    temp$25 := 0;
+    $return := temp$25;
+    return;
+  block4:
+  block2:
+    assert this1 != $null;
+    temp$36 := $heap[this1,InfeasibleCode01$InfeasibleCode01$bases234];
+    assert temp$36 != $null;
+    if ($heap[temp$36,$type] <: InfeasibleCode01 && InfeasibleCode01 <: $heap[temp$36,$type]) {
+        call temp$47, $exception := int$java.lang.Object$hashCode$41(temp$36);
+    }
+    assert other2 != $null;
+    temp$58 := $heap[other2,InfeasibleCode01$InfeasibleCode01$bases234];
+    assert temp$58 != $null;
+    if ($heap[temp$58,$type] <: InfeasibleCode01 && InfeasibleCode01 <: $heap[temp$58,$type]) {
+        call temp$69, $exception := int$java.lang.Object$hashCode$41(temp$58);
+    }
+    if (temp$47 != temp$69) {
+        goto block5;
+    }
+    goto block6;
+  block5:
+    temp$710 := 0;
+    $return := temp$710;
+    return;
+  block6:
+    temp$811 := 1;
+    $return := temp$811;
     return;
 }
 
-procedure java.lang.String$java.lang.String$substring$108($this:ref, $in_parameter__0:int, $in_parameter__1:int) returns ($return:ref, $exception:ref);
-    modifies ;
-    ensures $return != $null;
 
-var $stringSizeHeap : [ref]int;
-var $charArrayType : javaType;
-function $shrInt(x:int, y:int) returns ($ret:int);
-procedure void$java.lang.Object$$la$init$ra$$38($this:ref) returns ($exception:ref);
-    modifies ;
-
-const unique $alloc : Field bool extends  complete;
-function $refToBool(x:ref) returns ($ret:bool) { (if x == $null then false else true) }
-function $boolToInt(x:bool) returns ($ret:int) { (if x == true then 1 else 0) }
-var $intArrayType : javaType;
-procedure void$org.joogie.tests.InfeasibleCodeSnippets$$la$init$ra$$1868($this:ref) returns ($exception:ref)
-    modifies ;
-{
-    var $ex_return : bool;
-    var this14 : ref;
-
+implementation void$InfeasibleCode01$$la$init$ra$$1890($this:ref) returns ($exception:ref){
+    
+var this12 : ref;    
+var $ex_return : bool;
     assume $this != $null;
     $ex_return := false;
-    this14 := $this;
-    call $exception := void$java.lang.Object$$la$init$ra$$38(this14);
+    this12 := $this;
+    call $exception := void$java.lang.Object$$la$init$ra$$38(this12);
     return;
 }
 
-function $intToBool(x:int) returns ($ret:bool) { (if x == 0 then false else true) }
-type ref;
-const unique java.lang.Object : javaType extends  complete;
-const unique $null : ref extends  complete;
-function $realToInt(x:real) returns ($ret:int);
-var $boolArrayType : javaType;
-procedure java.lang.String$java.lang.String$toLowerCase$120($this:ref) returns ($return:ref, $exception:ref);
-    modifies ;
-    ensures $return != $null;
 
-var $boolArrHeap : [ref][int]bool;
-procedure java.lang.String$java.lang.Object$toString$44($this:ref) returns ($return:ref, $exception:ref);
-    ensures $return != $null;
-    modifies ;
-
-const unique java.lang.Throwable : javaType extends  unique java.io.Serializable, unique java.lang.Object complete;
-function $bitAnd(x:int, y:int) returns ($ret:int);
-const unique java.lang.RuntimeException : javaType extends  unique java.lang.Exception complete;
-type Field $GenericType__0;
-function $cmpBool(x:bool, y:bool) returns ($ret:int);
-function $arrayType(t:javaType) returns ($ret:javaType);
-var $refArrHeap : [ref][int]ref;
-procedure java.lang.String$org.joogie.tests.InfeasibleCodeSnippets$test2$1866($this:ref, $in_parameter__0:ref) returns ($return:ref, $exception:ref)
-    modifies $heap;
-{
-    var x7 : ref;
-    var this6 : ref;
-    var temp$08 : ref;
-    var $ex_return : bool;
-    var $fakelocal_0 : ref;
-
-    assume $this != $null;
-    $ex_return := false;
-    this6 := $this;
-    x7 := $in_parameter__0;
-    if (x7 != $null) {
-        $exception := $exception;
-    } else {
-        havoc $fakelocal_0;
-        assume !$heap[$fakelocal_0,$alloc];
-        $heap := $heap[$fakelocal_0,$alloc := true];
-        assume $fakelocal_0 != $null;
-        $heap := $heap[$fakelocal_0,$type := java.lang.NullPointerException];
-        $exception := $fakelocal_0;
-        $ex_return := true;
-        return;
-    }
-    if ($heap[x7,$type] <: java.lang.String && java.lang.String <: $heap[x7,$type]) {
-        call temp$08, $exception := java.lang.String$java.lang.Object$toString$44(x7);
-        assume temp$08 != $null;
-        assume $heap[temp$08,$type] <: java.lang.String;
-        assume java.lang.String <: $heap[temp$08,$type];
-    }
-    if ($heap[x7,$type] <: java.lang.Object && java.lang.Object <: $heap[x7,$type]) {
-        call temp$08, $exception := java.lang.String$java.lang.Object$toString$44(x7);
-        assume temp$08 != $null;
-        assume $heap[temp$08,$type] <: java.lang.String;
-        assume java.lang.String <: $heap[temp$08,$type];
-    }
-    $return := temp$08;
-    return;
-}
-
-function $shlInt(x:int, y:int) returns ($ret:int);
-var $byteArrayType : javaType;
-const unique java.lang.String : javaType extends  unique java.lang.Comparable, unique java.io.Serializable, unique java.lang.CharSequence, unique java.lang.Object complete;
-function $intToReal(x:int) returns ($ret:real);
-function $cmpReal(x:real, y:real) returns ($ret:int) { (if x > y then 1 else (if x < y then -1 else 0)) }
-function $ushrInt(x:int, y:int) returns ($ret:int);
-const unique java.io.Serializable : javaType extends  unique java.lang.Object complete;
-type void;
-const unique java.lang.NullPointerException : javaType extends  unique java.lang.RuntimeException complete;
-function $cmpRef(x:ref, y:ref) returns ($ret:int);
-function $xorInt(x:int, y:int) returns ($ret:int);
-procedure java.lang.String$java.lang.String$toUpperCase$122($this:ref) returns ($return:ref, $exception:ref);
-    ensures $return != $null;
-    modifies ;
-
-type javaType;
-const unique java.lang.CharSequence : javaType extends  unique java.lang.Object complete;
-var $heap : <$GenericType__0>[ref,Field $GenericType__0]$GenericType__0;
-var $realArrHeap : [ref][int]int;
-const unique java.lang.Comparable : javaType extends  unique java.lang.Object complete;
-function $bitOr(x:int, y:int) returns ($ret:int);
-const unique $type : Field javaType extends  complete;
-const unique java.lang.Exception : javaType extends  unique java.lang.Throwable complete;
-var $intArrHeap : [ref][int]int;
-const unique org.joogie.tests.InfeasibleCodeSnippets : javaType extends  unique java.lang.Object complete;
-function $cmpInt(x:int, y:int) returns ($ret:int) { (if x > y then 1 else (if x < y then -1 else 0)) }
-var $longArrayType : javaType;
-var $arrSizeHeap : [ref]int;
